Refactor memory implementations

examples/fib_heap/fib_heap_meldScript.sml
@@ -1,5 +1,5 @@
 (*
-  Memory Level Verification for Fibonacci heap
+  Memory Level Implementation and Verification for fts_meld
 *)
 Theory fib_heap_meld
 Ancestors
@@ -8,4 +8,184 @@ Ancestors
 Libs
   wordsLib helperLib
 
+
+
+Definition fib_heap_meld_def:
+  fib_heap_meld
+    (a1:'a word,a2:'a word,m:'a word -> 'a word_lab, dm: 'a word set)
+  =
+    if a2 = 0w then (a1,m,T) else
+(*    let c = in_mem a2 dm in *)
+    if a1 = 0w then (*list a is empty*)
+      (a2,m,T)
+    else
+      let (l_a1,c) = read_mem (a1 + before_off) m dm T in
+      let (l_a2,c) = read_mem (a2 + before_off) m dm c in
+
+      let (m,c) = write_mem (l_a1 + next_off) a2   m dm c in
+      let (m,c) = write_mem (a2 + before_off) l_a1 m dm c in
+      let (m,c) = write_mem (l_a2 + next_off) a1   m dm c in
+      let (m,c) = write_mem (a1 + before_off) l_a2 m dm c in
+
+      let (v_a2,c) = read_mem a2 m dm c in
+      let (v_a1,c) = read_mem a1 m dm c in
+      if v_a1 <=+ v_a2 then
+        (a1,m,c)
+      else
+        (a2,m,c)
+End
+
+
+Theorem fib_heap_meld_mem_thm:
+  !frame p fts1 fts2 fts' m dm.
+  fts_meld fts1 fts2 = fts' /\
+  (fts_mem (ann_fts p fts1) * fts_mem (ann_fts p fts2) * frame)
+    (fun2set (m,dm))
+  ==>
+  ?m'.
+  fib_heap_meld (head_key fts1,head_key fts2,m,dm) = (head_key fts',m',T) /\
+  (fts_mem (ann_fts p fts') * frame)
+    (fun2set (m',dm))
+Proof
+  rpt gen_tac >> disch_tac >> fs[] >>
+  Cases_on `fts1` >> Cases_on `fts2` >>
+  fs[fib_heap_meld_def,read_mem_def,write_mem_def,next_off_def,before_off_def,
+       head_key_def,head_key_t_def,fts_meld_def]
+  >- fs[fts_mem_def,ann_fts_def,SEP_CLAUSES]
+  >- (
+    Cases_on `h` >> gvs[] >>
+    fs[ann_fts_def, ann_fts_seg_def, last_key_def,fts_mem_def,
+       SEP_CLAUSES, head_key_def, ft_mem_def, new_anode_def,
+       new_dnode_def, head_key_t_def, ones_def, STAR_ASSOC] >>
+    full_simp_tac (std_ss ++ sep_cond_ss) [cond_STAR] >>
+    SEP_R_TAC >> simp[]
+    )
+  >- (
+    gvs[] >>
+    fs[fts_mem_def,ann_fts_def,SEP_CLAUSES,STAR_ASSOC]
+    ) >>
+  Cases_on `h` >> Cases_on `h'` >> gvs[] >>
+  rename[`(fts_mem (ann_fts p (FibTree k v l::t)) *
+     fts_mem (ann_fts p (FibTree k' v' l'::t')) * frame) (fun2set(m,dm))`] >>
+  fs[ann_fts_def, ann_fts_seg_def, last_key_def,last_key_t_def, fts_mem_def,
+     SEP_CLAUSES, head_key_def, ft_mem_def, new_anode_def,
+     new_dnode_def, head_key_t_def, ones_def, STAR_ASSOC] >>
+  full_simp_tac (std_ss ++ sep_cond_ss) [cond_STAR] >>
+  Cases_on `t` using SNOC_CASES >>
+  Cases_on `t'` using SNOC_CASES >>
+  fs[SNOC_APPEND,REVERSE_APPEND,fts_meld_def] >>
+  IF_CASES_TAC >>
+  SEP_R_TAC >> fs[head_key_t_def] >>
+  SEP_R_TAC >> simp[]
+  >- (
+    SEP_W_TAC >> simp[] >>
+    SEP_R_TAC >> fs[] >>
+    fs[ann_fts_def, ann_fts_seg_def, last_key_def,last_key_t_def, fts_mem_def,
+       SEP_CLAUSES, head_key_def, ft_mem_def, new_anode_def,
+       new_dnode_def, head_key_t_def, ones_def, STAR_ASSOC]
+    )
+  >- (
+    SEP_W_TAC >> simp[] >>
+    SEP_R_TAC >>
+    fs[ann_fts_def, ann_fts_seg_def, last_key_def,last_key_t_def, fts_mem_def,
+       SEP_CLAUSES, head_key_def, ft_mem_def, new_anode_def,
+       new_dnode_def, head_key_t_def, ones_def, STAR_ASSOC] >>
+    fs[AC STAR_ASSOC STAR_COMM]
+    )
+  >- (
+    Cases_on `x` >> fs[head_key_t_def] >>
+    fs[REVERSE_APPEND,ann_fts_seg_append_thm,fts_mem_append_thm] >>
+    fs[ann_fts_def, ann_fts_seg_def, last_key_def, last_key_t_def, fts_mem_def,
+       SEP_CLAUSES, head_key_def, ft_mem_def, new_anode_def,
+       new_dnode_def, head_key_t_def, ones_def, STAR_ASSOC] >>
+    SEP_R_TAC >>
+    SEP_W_TAC >> simp[] >>
+    SEP_R_TAC >>
+    fs[REVERSE_APPEND,ann_fts_seg_append_thm,fts_mem_append_thm,
+       ann_fts_def, ann_fts_seg_def, last_key_def,last_key_t_def, fts_mem_def,
+       SEP_CLAUSES, head_key_def, ft_mem_def, new_anode_def,
+       new_dnode_def, head_key_t_def, ones_def, STAR_ASSOC] >>
+    fs[head_key_t_pull_last_thm]
+    )
+  >- (
+    Cases_on `x` >> fs[head_key_t_def] >>
+    fs[REVERSE_APPEND,ann_fts_seg_append_thm,fts_mem_append_thm] >>
+    fs[ann_fts_def, ann_fts_seg_def, last_key_def, last_key_t_def, fts_mem_def,
+       SEP_CLAUSES, head_key_def, ft_mem_def, new_anode_def,
+       new_dnode_def, head_key_t_def, ones_def, STAR_ASSOC] >>
+    SEP_R_TAC >>
+    SEP_W_TAC >> simp[] >>
+    SEP_R_TAC >>
+    fs[REVERSE_APPEND,ann_fts_seg_append_thm,fts_mem_append_thm,
+       ann_fts_def, ann_fts_seg_def, last_key_def,last_key_t_def, fts_mem_def,
+       SEP_CLAUSES, head_key_def, ft_mem_def, new_anode_def,
+       new_dnode_def, head_key_t_def, ones_def, STAR_ASSOC] >>
+    fs[head_key_t_pull_last_thm,last_key_t_pull_thm,head_key_def,head_key_t_def] >>
+    fs[AC STAR_ASSOC STAR_COMM]
+    )
+  >- (
+    Cases_on `x` >> fs[head_key_t_def] >>
+    fs[REVERSE_APPEND,ann_fts_seg_append_thm,fts_mem_append_thm] >>
+    fs[ann_fts_def, ann_fts_seg_def, last_key_def, last_key_t_def, fts_mem_def,
+       SEP_CLAUSES, head_key_def, ft_mem_def, new_anode_def,
+       new_dnode_def, head_key_t_def, ones_def, STAR_ASSOC] >>
+    SEP_R_TAC >>
+    SEP_W_TAC >> simp[] >>
+    SEP_R_TAC >>
+    fs[REVERSE_APPEND,ann_fts_seg_append_thm,fts_mem_append_thm,
+       ann_fts_def, ann_fts_seg_def, last_key_def,last_key_t_def, fts_mem_def,
+       SEP_CLAUSES, head_key_def, ft_mem_def, new_anode_def,
+       new_dnode_def, head_key_t_def, ones_def, STAR_ASSOC] >>
+    fs[head_key_t_pull_last_thm,last_key_t_pull_thm,head_key_def,head_key_t_def] >>
+    fs[AC STAR_ASSOC STAR_COMM]
+    )
+  >- (
+    Cases_on `x` >> fs[head_key_t_def] >>
+    fs[REVERSE_APPEND,ann_fts_seg_append_thm,fts_mem_append_thm] >>
+    fs[ann_fts_def, ann_fts_seg_def, last_key_def, last_key_t_def, fts_mem_def,
+       SEP_CLAUSES, head_key_def, ft_mem_def, new_anode_def,
+       new_dnode_def, head_key_t_def, ones_def, STAR_ASSOC] >>
+    SEP_R_TAC >>
+    SEP_W_TAC >> simp[] >>
+    SEP_R_TAC >>
+    fs[REVERSE_APPEND,ann_fts_seg_append_thm,fts_mem_append_thm,
+       ann_fts_def, ann_fts_seg_def, last_key_def,last_key_t_def, fts_mem_def,
+       SEP_CLAUSES, head_key_def, ft_mem_def, new_anode_def,
+       new_dnode_def, head_key_t_def, ones_def, STAR_ASSOC] >>
+    fs[head_key_t_pull_last_thm,last_key_t_pull_thm,head_key_def,head_key_t_def] >>
+    fs[AC STAR_ASSOC STAR_COMM]
+    )
+  >- (
+    Cases_on `x` >> Cases_on `x'` >> fs[head_key_t_def] >>
+    fs[REVERSE_APPEND,ann_fts_seg_append_thm,fts_mem_append_thm] >>
+    fs[ann_fts_def, ann_fts_seg_def, last_key_def, last_key_t_def, fts_mem_def,
+       SEP_CLAUSES, head_key_def, ft_mem_def, new_anode_def,
+       new_dnode_def, head_key_t_def, ones_def, STAR_ASSOC] >>
+    SEP_R_TAC >>
+    SEP_W_TAC >> simp[] >>
+    SEP_R_TAC >>
+    fs[REVERSE_APPEND,ann_fts_seg_append_thm,fts_mem_append_thm,
+       ann_fts_def, ann_fts_seg_def, last_key_def,last_key_t_def, fts_mem_def,
+       SEP_CLAUSES, head_key_def, ft_mem_def, new_anode_def,
+       new_dnode_def, head_key_t_def, ones_def, STAR_ASSOC] >>
+    fs[head_key_t_pull_last_thm,last_key_t_pull_thm,head_key_def,head_key_t_def] >>
+    fs[head_key_t_append_thm,head_key_t_pull_last_thm] >>
+    fs[AC STAR_ASSOC STAR_COMM]
+    ) >>
+  Cases_on `x` >> Cases_on `x'` >> fs[head_key_t_def] >>
+  fs[REVERSE_APPEND,ann_fts_seg_append_thm,fts_mem_append_thm] >>
+  fs[ann_fts_def, ann_fts_seg_def, last_key_def, last_key_t_def, fts_mem_def,
+     SEP_CLAUSES, head_key_def, ft_mem_def, new_anode_def,
+     new_dnode_def, head_key_t_def, ones_def, STAR_ASSOC] >>
+  SEP_R_TAC >>
+  SEP_W_TAC >> simp[] >>
+  SEP_R_TAC >>
+  fs[REVERSE_APPEND,ann_fts_seg_append_thm,fts_mem_append_thm,
+     ann_fts_def, ann_fts_seg_def, last_key_def,last_key_t_def, fts_mem_def,
+     SEP_CLAUSES, head_key_def, ft_mem_def, new_anode_def,
+     new_dnode_def, head_key_t_def, ones_def, STAR_ASSOC] >>
+  fs[head_key_t_pull_last_thm,last_key_t_pull_thm,head_key_def,head_key_t_def] >>
+  fs[head_key_t_append_thm,head_key_t_pull_last_thm] >>
+  fs[AC STAR_ASSOC STAR_COMM]
+QED
 
