examples/fib_heap/README.md
@@ -1,10 +1,10 @@
 Verified version of the Fibonacci heap for use with Pancake
 
 [fib_heap_ext_minScript.sml](fib_heap_ext_minScript.sml):
-Memory Level Verification for the Extract Minimum Operation on a Fibonacci heap
+Memory Level Implementation and Verification for fts_ext_min
 
 [fib_heap_meldScript.sml](fib_heap_meldScript.sml):
-Memory Level Verification for Fibonacci heap
+Memory Level Implementation and Verification for fts_meld
 
 [fib_heap_panScript.sml](fib_heap_panScript.sml):
 fib_heap merge implementation in Pancake
